theories/Staging/NewShallow/IrisInstance.v
@@ -560,9 +560,9 @@ Module Type IrisAdequacy
       iMod (own_alloc ((● RegStore_to_map γ ⋅ ◯ RegStore_to_map γ ) : regUR)) as (spec_name) "[Hs1 Hs2]";
         first by apply auth_both_valid.
       pose proof (memΣ_GpreS (Σ := sailΣ) _) as mGS.
-      iMod (mem_inv_init (mGS := mGS)) as (memG) "[Hmem Rmem]".
+      iMod (mem_init (mGS := mGS)) as (memG) "[Hmem Rmem]".
       iModIntro.
-      iExists (fun σ _ => regs_inv (srGS := (SailRegGS _ spec_name)) (σ.1) ∗ mem_inv (σ.2))%I.
+      iExists (fun σ _ => regs_inv (srGS := (SailRegGS _ spec_name)) (σ.1) ∗ mem_state_interp (σ.2))%I.
       iExists _.
       iSplitR "Hs2 Rmem".
       * iFrame.
@@ -583,7 +583,7 @@ Module Type IrisAdequacy
     ⟨ γ, μ, δ, s ⟩ --->* ⟨ γ', μ', δ', s' ⟩ ->
     (forall `{sailGS Σ'},
         mem_res μ ∗ own_regstore γ ⊢ |={⊤}=> semWP s Q δ
-          ∗ (mem_inv μ' ={⊤,∅}=∗ ⌜φ⌝)
+          ∗ (mem_state_interp μ' ={⊤,∅}=∗ ⌜φ⌝)
     )%I -> φ.
   Proof.
     (* intros steps trips. *)
@@ -595,7 +595,7 @@ Module Type IrisAdequacy
     iMod (own_alloc ((● RegStore_to_map γ ⋅ ◯ RegStore_to_map γ ) : regUR)) as (spec_name) "[Hs1 Hs2]";
         first by apply auth_both_valid.
     pose proof (memΣ_GpreS (Σ := sailΣ) _) as mGS.
-    iMod (mem_inv_init (mGS := mGS)) as (memG) "[Hmem Rmem]".
+    iMod (mem_init (mGS := mGS)) as (memG) "[Hmem Rmem]".
     pose (regsG := {| reg_inG := @reg_pre_inG sailΣ (@subG_sailGpreS sailΣ (subG_refl sailΣ)); reg_gv_name := spec_name |}).
     pose (sailG := SailGS Hinv regsG memG).
     iMod (trips sailΣ sailG with "[Rmem Hs2]") as "[trips Hφ]".
@@ -605,7 +605,7 @@ Module Type IrisAdequacy
       eapply finite.NoDup_enum.
     }
     iModIntro.
-    iExists (fun σ _ _ _ => regs_inv (srGS := (SailRegGS _ spec_name)) (σ.1) ∗ mem_inv (σ.2))%I.
+    iExists (fun σ _ _ _ => regs_inv (srGS := (SailRegGS _ spec_name)) (σ.1) ∗ mem_state_interp (σ.2))%I.
     iExists [ fun v => Q _ sailG (valconf_val v) (valconf_store v) ]%list.
     iExists _.
     iExists _.
